Weidenbach_Book/IsaSAT_VMTF_LLVM.thy
@@ -11,8 +11,6 @@ begin
 (*declare is_None_def[simp del] *)
 
 
-
-
 (*
 lemma VMTF_Node_ref[sepref_fr_rules]:
   \<open>(uncurry2 (return ooo VMTF_Node), uncurry2 (RETURN ooo VMTF_Node)) \<in>
@@ -43,21 +41,19 @@ lemma get_prev_ref[sepref_fr_rules]:
 
 sepref_definition atoms_hash_del_code
   is \<open>uncurry (RETURN oo atoms_hash_del)\<close>
-  :: \<open>[uncurry atoms_hash_del_pre]\<^sub>a uint32_nat_assn\<^sup>k *\<^sub>a (atoms_hash_assn)\<^sup>d \<rightarrow> atoms_hash_assn\<close>
+  :: \<open>[uncurry atoms_hash_del_pre]\<^sub>a atom_assn\<^sup>k *\<^sub>a (atoms_hash_assn)\<^sup>d \<rightarrow> atoms_hash_assn\<close>
   unfolding atoms_hash_del_def atoms_hash_del_pre_def
-  apply (rewrite at \<open>list_update _ \<hole>\<close> annot_unat_snat_upcast[where 'l=64])
+  apply annot_all_atm_idxs
   by sepref
 
 declare atoms_hash_del_code.refine[sepref_fr_rules]
 sepref_definition (in -) atoms_hash_insert_code
   is \<open>uncurry (RETURN oo atoms_hash_insert)\<close>
   :: \<open>[uncurry atms_hash_insert_pre]\<^sub>a
-      uint32_nat_assn\<^sup>k *\<^sub>a (distinct_atoms_assn)\<^sup>d \<rightarrow>  distinct_atoms_assn\<close>
+      atom_assn\<^sup>k *\<^sub>a (distinct_atoms_assn)\<^sup>d \<rightarrow>  distinct_atoms_assn\<close>
   unfolding atoms_hash_insert_def atms_hash_insert_pre_def
-  supply [simp] = uint32_max_def max_snat_def
   supply [[goals_limit=1]]
-  apply (rewrite at \<open>list_update _ \<hole>\<close> annot_unat_snat_upcast[where 'l=64])
-  apply (rewrite at \<open>_ ! \<hole>\<close> annot_unat_snat_upcast[where 'l=64])
+  apply annot_all_atm_idxs
   by sepref
 
 declare atoms_hash_insert_code.refine[sepref_fr_rules]
@@ -116,13 +112,13 @@ lemma hfref_refine_with_pre:
   
 lemma isa_vmtf_en_dequeue_preI:
   assumes "isa_vmtf_en_dequeue_pre ((M,L),(ns, m, fst_As, lst_As, next_search))"  
-  shows "fst_As < length ns" "L < length ns" "m < max_snat 64"
+  shows "fst_As < length ns" "L < length ns" "Suc m < max_unat 64"
     and "get_next (ns!L) = Some i \<longrightarrow> i < length ns"
     and "fst_As \<noteq> lst_As \<longrightarrow> get_prev (ns ! lst_As) \<noteq> None"
     and "get_next (ns ! fst_As) \<noteq> None \<longrightarrow> get_prev (ns ! lst_As) \<noteq> None"
   using assms
   unfolding isa_vmtf_en_dequeue_pre_def vmtf_dequeue_pre_def
-  apply (auto simp: max_snat_def sint64_max_def)
+  apply (auto simp: max_unat_def uint64_max_def sint64_max_def)
   done
   
   
@@ -142,7 +138,7 @@ lemma isa_vmtf_en_dequeue_alt_def2:
       let ns = ns_vmtf_dequeue L ns;
       ASSERT (defined_atm_pol_pre M L);
       let de = (defined_atm_pol M L);
-      ASSERT (m < max_snat 64);
+      ASSERT (Suc m < max_unat 64);
       case fst_As of
         None \<Rightarrow> RETURN
           (ns[L := VMTF_Node m fst_As None], m + 1, L, L,
@@ -185,9 +181,9 @@ sepref_register 1 0
 
 lemma vmtf_en_dequeue_fast_codeI:
   assumes "isa_vmtf_en_dequeue_pre ((M, L),(ns,m,fst_As, lst_As, next_search))"
-  shows "m < max_snat 64"
+  shows "Suc m < max_unat 64"
   using assms
-  unfolding isa_vmtf_en_dequeue_pre_def max_snat_def sint64_max_def
+  unfolding isa_vmtf_en_dequeue_pre_def max_unat_def uint64_max_def
   by auto
   
   
@@ -202,7 +198,6 @@ sepref_definition vmtf_en_dequeue_fast_code
   apply (rule hfref_refine_with_pre[OF isa_vmtf_en_dequeue_alt_def2], assumption)
   
   supply [[goals_limit = 1]]
-  supply [simp] = max_unat_def max_snat_def
   unfolding isa_vmtf_en_dequeue_alt_def2 case_option_split eq_Some_iff 
   apply (rewrite in "if \<hole> then get_next _ else _" short_circuit_conv)
   apply annot_all_atm_idxs    
@@ -217,8 +212,6 @@ sepref_definition vmtf_rescale_code
    is \<open>vmtf_rescale\<close>
    :: \<open>vmtf_assn\<^sup>d \<rightarrow>\<^sub>a vmtf_assn\<close>
   supply [[goals_limit = 1]]
-  supply [simp] = uint32_max_def max_snat_def max_unat_def
-  
   supply vmtf_en_dequeue_pre_def[simp]
   unfolding vmtf_rescale_alt_def update_stamp.simps
   unfolding atom.fold_option
@@ -233,18 +226,19 @@ declare vmtf_rescale_code.refine[sepref_fr_rules]
 sepref_definition partition_vmtf_nth_code
    is \<open>uncurry3 partition_vmtf_nth\<close>
    :: \<open>[\<lambda>(((ns, _), hi), xs). (\<forall>x\<in>set xs. x < length ns) \<and> length xs \<le> uint32_max]\<^sub>a
-  (array_assn vmtf_node_assn)\<^sup>k *\<^sub>a sint64_nat_assn\<^sup>k *\<^sub>a sint64_nat_assn\<^sup>k *\<^sub>a (arl64_assn uint32_nat_assn)\<^sup>d \<rightarrow>
-  arl64_assn uint32_nat_assn *a sint64_nat_assn\<close>
+  (array_assn vmtf_node_assn)\<^sup>k *\<^sub>a sint64_nat_assn\<^sup>k *\<^sub>a sint64_nat_assn\<^sup>k *\<^sub>a (arl64_assn atom_assn)\<^sup>d \<rightarrow>
+  arl64_assn atom_assn *a sint64_nat_assn\<close>
   unfolding partition_vmtf_nth_def
     partition_main_def choose_pivot3_def
     convert_swap gen_swap
     
-  apply (rewrite at "stamp (_!\<hole>)" annot_unat_snat_upcast[where 'l=64])  
-  apply (rewrite at "stamp (_!\<hole>)" in "if \<hole> then _ else _" annot_unat_snat_upcast[where 'l=64])  
   apply (annot_snat_const "TYPE(64)")  
   supply [[goals_limit = 1]]
   supply [simp] = max_snat_def uint32_max_def
   supply partition_vmtf_nth_code_helper3[intro] partition_main_inv_def[simp]
+  apply (rewrite at \<open>_ ! _\<close> at \<open>stamp ( _ ! \<hole>)\<close> value_of_atm_def[symmetric])
+  apply (rewrite at \<open>stamp ( _ ! \<hole>)\<close> in \<open>If \<hole> _\<close> value_of_atm_def[symmetric])
+  unfolding index_of_atm_def[symmetric]
   by sepref
 
 declare partition_vmtf_nth_code.refine[sepref_fr_rules]
@@ -264,8 +258,8 @@ sepref_register partition_between_ref
 sepref_definition (in -) partition_between_ref_vmtf_code
    is \<open>uncurry3 partition_between_ref_vmtf\<close>
    :: \<open>[\<lambda>(((vm), _), remove). (\<forall>x\<in>#mset remove. x < length (fst vm)) \<and> length remove \<le> uint32_max]\<^sub>a
-      (array_assn vmtf_node_assn)\<^sup>k *\<^sub>a sint64_nat_assn\<^sup>k *\<^sub>a sint64_nat_assn\<^sup>k *\<^sub>a (arl64_assn uint32_nat_assn)\<^sup>d  \<rightarrow>
-       arl64_assn uint32_nat_assn *a sint64_nat_assn\<close>
+      (array_assn vmtf_node_assn)\<^sup>k *\<^sub>a sint64_nat_assn\<^sup>k *\<^sub>a sint64_nat_assn\<^sup>k *\<^sub>a (arl64_assn atom_assn)\<^sup>d  \<rightarrow>
+       arl64_assn atom_assn *a sint64_nat_assn\<close>
   supply [[goals_limit=1]]
   unfolding quicksort_vmtf_nth_def partition_vmtf_nth_def[symmetric]
     quicksort_vmtf_nth_ref_def List.null_def quicksort_ref_def
@@ -273,9 +267,13 @@ sepref_definition (in -) partition_between_ref_vmtf_code
     partition_between_ref_def 
     partition_vmtf_nth_def[symmetric] choose_pivot3_def
     convert_swap gen_swap
+  apply (rewrite at \<open>_ ! _\<close> at \<open>stamp ( _ ! \<hole>)\<close> value_of_atm_def[symmetric])
+  apply (rewrite at \<open>let _ = _; _ = stamp ( _ ! \<hole>) in _\<close> value_of_atm_def[symmetric])
+  apply (rewrite at \<open>let _ = _; _ = _; _ = stamp ( _ ! \<hole>) in _\<close> value_of_atm_def[symmetric])
+  unfolding index_of_atm_def[symmetric]
   apply (annot_snat_const "TYPE(64)")
-  apply (rewrite at "_!_" at "stamp (_!\<hole>)" annot_unat_snat_upcast[where 'l=64])+  
-  by sepref  
+  by sepref
+
 sepref_register partition_between_ref_vmtf quicksort_vmtf_nth_ref
 declare partition_between_ref_vmtf_code.refine[sepref_fr_rules]
 
@@ -283,11 +281,11 @@ lemma quicksort_vmtf_nth_ref_code_avoid_minus: "p - (1::nat) \<le> lo \<longleft
 sepref_definition (in -) quicksort_vmtf_nth_ref_code
    is \<open>uncurry3 quicksort_vmtf_nth_ref\<close>
    :: \<open>[\<lambda>((vm, _), remove). (\<forall>x\<in>#mset remove. x < length (fst vm)) \<and> length remove \<le> uint32_max]\<^sub>a
-      (array_assn vmtf_node_assn)\<^sup>k *\<^sub>a sint64_nat_assn\<^sup>k *\<^sub>a sint64_nat_assn\<^sup>k *\<^sub>a (arl64_assn uint32_nat_assn)\<^sup>d  \<rightarrow>
-       arl64_assn uint32_nat_assn\<close>
+      (array_assn vmtf_node_assn)\<^sup>k *\<^sub>a sint64_nat_assn\<^sup>k *\<^sub>a sint64_nat_assn\<^sup>k *\<^sub>a (arl64_assn atom_assn)\<^sup>d  \<rightarrow>
+       arl64_assn atom_assn\<close>
   unfolding quicksort_vmtf_nth_def partition_vmtf_nth_def[symmetric]
     quicksort_vmtf_nth_ref_def List.null_def quicksort_ref_def
-    length_0_conv[symmetric] (*length_uint32_nat_def[symmetric]*)
+    length_0_conv[symmetric]
    partition_vmtf_nth_def[symmetric]
    partition_between_ref_vmtf_def[symmetric]
    partition_vmtf_nth_def[symmetric]
@@ -302,8 +300,8 @@ declare quicksort_vmtf_nth_ref_code.refine[sepref_fr_rules]
 sepref_definition (in -) quicksort_vmtf_nth_code
    is \<open>uncurry quicksort_vmtf_nth\<close>
    :: \<open>[\<lambda>(vm, remove). (\<forall>x\<in>#mset remove. x < length (fst vm)) \<and> length remove \<le> uint32_max]\<^sub>a
-      vmtf_assn\<^sup>k *\<^sub>a (arl64_assn uint32_nat_assn)\<^sup>d  \<rightarrow>
-       arl64_assn uint32_nat_assn\<close>
+      vmtf_assn\<^sup>k *\<^sub>a (arl64_assn atom_assn)\<^sup>d  \<rightarrow>
+       arl64_assn atom_assn\<close>
   unfolding quicksort_vmtf_nth_def partition_vmtf_nth_def[symmetric]
     full_quicksort_ref_def List.null_def 
     length_0_conv[symmetric] 
@@ -318,7 +316,7 @@ declare quicksort_vmtf_nth_code.refine[sepref_fr_rules]
 lemma quicksort_vmtf_nth_code_reorder_list[sepref_fr_rules]:
    \<open>(uncurry quicksort_vmtf_nth_code, uncurry reorder_list) \<in>
       [\<lambda>((a, _), b). (\<forall>x\<in>set b. x < length a) \<and> length b \<le> uint32_max]\<^sub>a
-      vmtf_assn\<^sup>k *\<^sub>a (arl64_assn uint32_nat_assn)\<^sup>d \<rightarrow> arl64_assn uint32_nat_assn\<close>
+      vmtf_assn\<^sup>k *\<^sub>a (arl64_assn atom_assn)\<^sup>d \<rightarrow> arl64_assn atom_assn\<close>
       supply [[show_types]]
   using quicksort_vmtf_nth_code.refine[FCOMP quicksort_vmtf_nth_reorder[unfolded convert_fref]]
   by auto
@@ -328,53 +326,45 @@ sepref_register isa_vmtf_enqueue
 lemma uint64_nal_rel_le_uint64_max: \<open>(a, b) \<in> uint64_nat_rel \<Longrightarrow> b \<le> uint64_max\<close>
   by (auto simp: uint64_nat_rel_def br_def nat_of_uint64_le_uint64_max)
 *)  
+lemma emptied_list_alt_def: \<open>emptied_list xs = take 0 xs\<close>
+  by (auto simp: emptied_list_def)
 
+sepref_definition current_stamp_impl
+  is \<open>RETURN o current_stamp\<close>
+  :: \<open>vmtf_assn\<^sup>k \<rightarrow>\<^sub>a uint64_nat_assn\<close>
+  unfolding current_stamp_alt_def
+  by sepref
 
-
-(*
-(*TODO deduplitacte*)
-text \<open>This functions deletes all elements of a resizable array, without resizing it.\<close>
-definition emptied_arl :: \<open>'a array_list32 \<Rightarrow> 'a array_list32\<close> where
-\<open>emptied_arl = (\<lambda>(a, n). (a, 0))\<close>
-
-lemma emptied_arl_refine[sepref_fr_rules]:
-  \<open>(return o emptied_arl, RETURN o emptied_list) \<in> (arl64_assn R)\<^sup>d \<rightarrow>\<^sub>a arl64_assn R\<close>
-  unfolding emptied_arl_def emptied_list_def
-  by sepref_to_hoare (sep_auto simp: arl64_assn_def hr_comp_def is_array_list32_def)
-*)  
+lemmas [sepref_fr_rules] = current_stamp_impl.refine
 
 sepref_register isa_vmtf_en_dequeue
 
 sepref_definition isa_vmtf_flush_fast_code
    is \<open>uncurry isa_vmtf_flush_int\<close>
-   :: \<open>trail_pol_fast_assn\<^sup>k *\<^sub>a (vmtf_assn *a (arl64_assn uint32_nat_assn *a atoms_hash_assn))\<^sup>d \<rightarrow>\<^sub>a
-        (vmtf_assn *a (arl64_assn uint32_nat_assn *a atoms_hash_assn))\<close>
-  supply [[goals_limit = 1]] 
-  unfolding vmtf_flush_def PR_CONST_def isa_vmtf_flush_int_def current_stamp_def[symmetric]
-  unfolding current_stamp_alt_def
-  apply (rewrite at \<open>sint64_max\<close> annot_snat_snat_upcast)
-  apply (rewrite at \<open>length _ + \<hole>\<close> nat_of_uint64_conv_def[symmetric])
-  
-(*  apply (rewrite at \<open>If (\<hole> \<ge> _)\<close> uint64_of_uint32_conv_def[symmetric])
-  apply (rewrite at \<open>length _ + \<hole>\<close> nat_of_uint64_conv_def[symmetric])
-*)  
-  apply sepref_dbg_keep
-  apply sepref_dbg_trans_keep
-  apply sepref_dbg_trans_step_keep
-  find_theorems current_stamp
-  
+   :: \<open>trail_pol_fast_assn\<^sup>k *\<^sub>a (vmtf_remove_assn)\<^sup>d \<rightarrow>\<^sub>a
+        vmtf_remove_assn\<close>
+  supply [[goals_limit = 1]]
+  unfolding vmtf_flush_def PR_CONST_def isa_vmtf_flush_int_def
+    current_stamp_def[symmetric] emptied_list_alt_def
+    vmtf_remove_assn_def
+  apply (rewrite at \<open>If (_ - _ \<le> \<hole>) _ _\<close> annot_snat_unat_conv)
+  apply (rewrite at \<open>WHILEIT _ (\<lambda>(_, _, _)._ < \<hole>)\<close> annot_snat_unat_conv)
+  apply (rewrite at \<open>isa_vmtf_en_dequeue _ (_ ! \<hole>)\<close> annot_unat_snat_conv)
+  apply (rewrite at \<open>atoms_hash_del (_ ! \<hole>)\<close> annot_unat_snat_conv)
+  apply (rewrite at \<open>take \<hole> _\<close> snat_const_fold[where 'a=64])
+  apply (annot_unat_const "TYPE(64)")
+  by sepref
 
-declare isa_vmtf_flush_code.refine[sepref_fr_rules]
-  isa_vmtf_flush_fast_code.refine[sepref_fr_rules]
+declare isa_vmtf_flush_fast_code.refine[sepref_fr_rules]
 
 sepref_register isa_vmtf_mark_to_rescore
 sepref_definition isa_vmtf_mark_to_rescore_code
   is \<open>uncurry (RETURN oo isa_vmtf_mark_to_rescore)\<close>
   :: \<open>[uncurry isa_vmtf_mark_to_rescore_pre]\<^sub>a
-     uint32_nat_assn\<^sup>k *\<^sub>a vmtf_remove_assn\<^sup>d \<rightarrow> vmtf_remove_assn\<close>
+     atom_assn\<^sup>k *\<^sub>a vmtf_remove_assn\<^sup>d \<rightarrow> vmtf_remove_assn\<close>
   supply [[goals_limit=1]] option.splits[split] vmtf_def[simp] in_\<L>\<^sub>a\<^sub>l\<^sub>l_atm_of_in_atms_of_iff[simp]
     neq_NilE[elim!] literals_are_in_\<L>\<^sub>i\<^sub>n_add_mset[simp]
-  unfolding isa_vmtf_mark_to_rescore_pre_def isa_vmtf_mark_to_rescore_def
+  unfolding isa_vmtf_mark_to_rescore_pre_def isa_vmtf_mark_to_rescore_def vmtf_remove_assn_def
   by sepref
 
 declare isa_vmtf_mark_to_rescore_code.refine[sepref_fr_rules]
@@ -383,40 +373,34 @@ sepref_register isa_vmtf_unset
 sepref_definition isa_vmtf_unset_code
   is \<open>uncurry (RETURN oo isa_vmtf_unset)\<close>
   :: \<open>[uncurry vmtf_unset_pre]\<^sub>a
-     uint32_nat_assn\<^sup>k *\<^sub>a vmtf_remove_assn\<^sup>d \<rightarrow> vmtf_remove_assn\<close>
+     atom_assn\<^sup>k *\<^sub>a vmtf_remove_assn\<^sup>d \<rightarrow> vmtf_remove_assn\<close>
   supply [[goals_limit=1]] option.splits[split] vmtf_def[simp] in_\<L>\<^sub>a\<^sub>l\<^sub>l_atm_of_in_atms_of_iff[simp]
     neq_NilE[elim!] literals_are_in_\<L>\<^sub>i\<^sub>n_add_mset[simp]
-  unfolding isa_vmtf_unset_def vmtf_unset_pre_def
+  unfolding isa_vmtf_unset_def vmtf_unset_pre_def vmtf_remove_assn_def atom.fold_option
   apply (rewrite in \<open>If (_ \<or> _)\<close> short_circuit_conv)
+  apply annot_all_atm_idxs
   by sepref
 
-declare isa_vmtf_unset_code.refine[sepref_fr_rules]
+lemmas [sepref_fr_rules] = isa_vmtf_mark_to_rescore_code.refine
+   isa_vmtf_unset_code.refine
+
+lemma isa_vmtf_mark_to_rescore_and_unsetI:  \<open>
+     atms_hash_insert_pre ak (ad, ba) \<Longrightarrow>
+       isa_vmtf_mark_to_rescore_pre ak ((a, aa, ab, ac, Some ak'), ad, ba)\<close>
+  by (auto simp: isa_vmtf_mark_to_rescore_pre_def)
 
 sepref_definition vmtf_mark_to_rescore_and_unset_code
   is \<open>uncurry (RETURN oo isa_vmtf_mark_to_rescore_and_unset)\<close>
   :: \<open>[isa_vmtf_mark_to_rescore_and_unset_pre]\<^sub>a
-      uint32_nat_assn\<^sup>k *\<^sub>a vmtf_remove_assn\<^sup>d \<rightarrow> vmtf_remove_assn\<close>
+      atom_assn\<^sup>k *\<^sub>a vmtf_remove_assn\<^sup>d \<rightarrow> vmtf_remove_assn\<close>
   supply image_image[simp] uminus_\<A>\<^sub>i\<^sub>n_iff[iff] in_diffD[dest] option.splits[split]
-    if_splits[split] isa_vmtf_unset_def[simp]
+    if_splits[split] isa_vmtf_unset_def[simp] isa_vmtf_mark_to_rescore_and_unsetI[intro!]
   supply [[goals_limit=1]]
-  unfolding isa_vmtf_mark_to_rescore_and_unset_def isa_vmtf_mark_to_rescore_def
+  unfolding isa_vmtf_mark_to_rescore_and_unset_def isa_vmtf_mark_to_rescore_and_unset_pre_def
     save_phase_def isa_vmtf_mark_to_rescore_and_unset_pre_def
   by sepref
 
 declare vmtf_mark_to_rescore_and_unset_code.refine[sepref_fr_rules]
-sepref_definition find_decomp_wl_imp_code
-  is \<open>uncurry2 (isa_find_decomp_wl_imp)\<close>
-  :: \<open>[\<lambda>((M, lev), vm). True]\<^sub>a trail_pol_assn\<^sup>d *\<^sub>a uint32_nat_assn\<^sup>k *\<^sub>a vmtf_remove_assn\<^sup>d
-    \<rightarrow> trail_pol_assn *a vmtf_remove_assn\<close>
-  unfolding isa_find_decomp_wl_imp_def get_maximum_level_remove_def[symmetric] PR_CONST_def
-    trail_pol_conv_to_no_CS_def
-  supply [[goals_limit=1]] literals_are_in_\<L>\<^sub>i\<^sub>n_add_mset[simp] trail_conv_to_no_CS_def[simp]
-    lit_of_hd_trail_def[simp]
-  supply uint32_nat_assn_one[sepref_fr_rules] vmtf_unset_pre_def[simp]
-  supply uint32_nat_assn_minus[sepref_fr_rules]
-  by sepref
-
-declare find_decomp_wl_imp_code.refine[sepref_fr_rules]
 
 sepref_definition find_decomp_wl_imp_fast_code
   is \<open>uncurry2 (isa_find_decomp_wl_imp)\<close>
@@ -426,40 +410,24 @@ sepref_definition find_decomp_wl_imp_fast_code
     trail_pol_conv_to_no_CS_def
   supply trail_conv_to_no_CS_def[simp] lit_of_hd_trail_def[simp]
   supply [[goals_limit=1]] literals_are_in_\<L>\<^sub>i\<^sub>n_add_mset[simp]
-  supply uint32_nat_assn_one[sepref_fr_rules] vmtf_unset_pre_def[simp]
-  supply uint32_nat_assn_minus[sepref_fr_rules]
+  supply vmtf_unset_pre_def[simp]
+  apply (rewrite at \<open>let _ = _ - \<hole> in _\<close> annot_unat_snat_upcast[where 'l=64])
+  apply (annot_snat_const "TYPE(64)")
   by sepref
 
 declare find_decomp_wl_imp_fast_code.refine[sepref_fr_rules]
 
-sepref_definition vmtf_rescore_code
-  is \<open>uncurry3 isa_vmtf_rescore\<close>
-  :: \<open>(array_assn unat_lit_assn)\<^sup>k *\<^sub>a trail_pol_assn\<^sup>k *\<^sub>a vmtf_remove_assn\<^sup>d *\<^sub>a phase_saver_conc\<^sup>d \<rightarrow>\<^sub>a
-       vmtf_remove_assn *a phase_saver_conc\<close>
-  unfolding isa_vmtf_rescore_body_def[abs_def] PR_CONST_def isa_vmtf_rescore_def
-  supply [[goals_limit = 1]] fold_is_None[simp]
-  by sepref
-
 sepref_definition vmtf_rescore_fast_code
   is \<open>uncurry3 isa_vmtf_rescore\<close>
-  :: \<open>(array_assn unat_lit_assn)\<^sup>k *\<^sub>a trail_pol_fast_assn\<^sup>k *\<^sub>a vmtf_remove_assn\<^sup>d *\<^sub>a phase_saver_conc\<^sup>d \<rightarrow>\<^sub>a
-       vmtf_remove_assn *a phase_saver_conc\<close>
+  :: \<open>(arl64_assn unat_lit_assn)\<^sup>k *\<^sub>a trail_pol_fast_assn\<^sup>k *\<^sub>a vmtf_remove_assn\<^sup>d *\<^sub>a phase_saver_assn\<^sup>d \<rightarrow>\<^sub>a
+       vmtf_remove_assn *a phase_saver_assn\<close>
   unfolding isa_vmtf_rescore_body_def[abs_def] PR_CONST_def isa_vmtf_rescore_def
   supply [[goals_limit = 1]] fold_is_None[simp]
+  apply (annot_snat_const "TYPE(64)")
   by sepref
 
 declare
-  vmtf_rescore_code.refine[sepref_fr_rules]
   vmtf_rescore_fast_code.refine[sepref_fr_rules]
-
-sepref_definition find_decomp_wl_imp'_code
-  is \<open>uncurry find_decomp_wl_st_int\<close>
-  :: \<open>uint32_nat_assn\<^sup>k *\<^sub>a isasat_unbounded_assn\<^sup>d  \<rightarrow>\<^sub>a isasat_unbounded_assn\<close>
-  unfolding find_decomp_wl_st_int_def PR_CONST_def isasat_unbounded_assn_def
-  supply [[goals_limit = 1]]
-  by sepref
-
-declare find_decomp_wl_imp'_code.refine[sepref_fr_rules]
 
 sepref_definition find_decomp_wl_imp'_fast_code
   is \<open>uncurry find_decomp_wl_st_int\<close>
@@ -470,58 +438,27 @@ sepref_definition find_decomp_wl_imp'_fast_code
   by sepref
 
 declare find_decomp_wl_imp'_fast_code.refine[sepref_fr_rules]
-sepref_definition vmtf_mark_to_rescore_clause_code
-  is \<open>uncurry2 (isa_vmtf_mark_to_rescore_clause)\<close>
-  :: \<open>arena_assn\<^sup>k *\<^sub>a nat_assn\<^sup>k *\<^sub>a vmtf_remove_assn\<^sup>d \<rightarrow>\<^sub>a vmtf_remove_assn\<close>
-  supply [[goals_limit=1]]
-  unfolding isa_vmtf_mark_to_rescore_clause_def PR_CONST_def
-  by sepref
 
-declare vmtf_mark_to_rescore_clause_code.refine[sepref_fr_rules]
 
-sepref_definition vmtf_mark_to_rescore_also_reasons_code
-  is \<open>uncurry3 (isa_vmtf_mark_to_rescore_also_reasons)\<close>
-  :: \<open>trail_pol_assn\<^sup>k *\<^sub>a arena_assn\<^sup>k *\<^sub>a (arl64_assn unat_lit_assn)\<^sup>k *\<^sub>a vmtf_remove_assn\<^sup>d \<rightarrow>\<^sub>a vmtf_remove_assn\<close>
-  supply image_image[simp] uminus_\<A>\<^sub>i\<^sub>n_iff[iff] in_diffD[dest] option.splits[split]
-    in_\<L>\<^sub>a\<^sub>l\<^sub>l_atm_of_\<A>\<^sub>i\<^sub>n[simp]
-  supply [[goals_limit=1]]
-  unfolding isa_vmtf_mark_to_rescore_also_reasons_def PR_CONST_def
-  unfolding while_eq_nfoldli[symmetric]
-  apply (subst while_upt_while_direct, simp)
-  apply (rewrite at \<open>(\<hole>, _)\<close> zero_uint32_nat_def[symmetric])
-  unfolding one_uint32_nat_def[symmetric] nres_monad3
-  by sepref
-
-declare vmtf_mark_to_rescore_also_reasons_code.refine[sepref_fr_rules]
-
-(*TODO kill and ann an imp_for64*)
-sepref_definition (in-) isa_arena_lit_fast_code2
-  is \<open>uncurry isa_arena_lit\<close>
-  :: \<open>(arl64_assn uint32_assn)\<^sup>k *\<^sub>a nat_assn\<^sup>k \<rightarrow>\<^sub>a uint32_assn\<close>
-  supply arena_el_assn_alt_def[symmetric, simp] sum_uint64_assn[sepref_fr_rules]
-  unfolding isa_arena_lit_def
-  by sepref
-
-declare isa_arena_lit_fast_code.refine
-
-lemma isa_arena_lit_fast_code_refine[sepref_fr_rules]:
-  \<open>(uncurry isa_arena_lit_fast_code2, uncurry (RETURN \<circ>\<circ> arena_lit))
-  \<in> [uncurry arena_lit_pre]\<^sub>a
-    arena_fast_assn\<^sup>k *\<^sub>a nat_assn\<^sup>k \<rightarrow> unat_lit_assn\<close>
-  using isa_arena_lit_fast_code2.refine[FCOMP isa_arena_lit_arena_lit[unfolded convert_fref]]
-  unfolding hr_comp_assoc[symmetric] uncurry_def list_rel_compp
-  by (simp add: arl64_assn_comp)
-(*ENd Move*)
+lemma (in -) arena_is_valid_clause_idx_le_uint64_max:
+  \<open>arena_is_valid_clause_idx be bd \<Longrightarrow>
+    length be \<le> sint64_max \<Longrightarrow>
+   bd + arena_length be bd < max_snat 64\<close>
+  \<open>arena_is_valid_clause_idx be bd \<Longrightarrow> length be \<le> sint64_max \<Longrightarrow>
+   bd < max_snat 64\<close>
+  using arena_lifting(10)[of be _ _ bd] unfolding max_snat_def sint64_max_def
+  by (fastforce simp: arena_lifting arena_is_valid_clause_idx_def)+
 
 sepref_definition vmtf_mark_to_rescore_clause_fast_code
   is \<open>uncurry2 (isa_vmtf_mark_to_rescore_clause)\<close>
-  :: \<open>[\<lambda>((N, _), _). length N \<le> uint64_max]\<^sub>a
-       arena_fast_assn\<^sup>k *\<^sub>a uint64_nat_assn\<^sup>k *\<^sub>a vmtf_remove_assn\<^sup>d \<rightarrow> vmtf_remove_assn\<close>
+  :: \<open>[\<lambda>((N, _), _). length N \<le> sint64_max]\<^sub>a
+       arena_fast_assn\<^sup>k *\<^sub>a sint64_nat_assn\<^sup>k *\<^sub>a vmtf_remove_assn\<^sup>d \<rightarrow> vmtf_remove_assn\<close>
   supply [[goals_limit=1]] arena_is_valid_clause_idx_le_uint64_max[intro]
-  unfolding isa_vmtf_mark_to_rescore_clause_def PR_CONST_def nat_of_uint64_conv_def
+  unfolding isa_vmtf_mark_to_rescore_clause_def PR_CONST_def
   unfolding while_eq_nfoldli[symmetric]
   apply (subst while_upt_while_direct, simp)
-  unfolding one_uint64_nat_def[symmetric] nres_monad3 zero_uint64_nat_def[symmetric]
+  unfolding nres_monad3
+  apply (annot_snat_const "TYPE(64)")
   by sepref
 
 declare vmtf_mark_to_rescore_clause_fast_code.refine[sepref_fr_rules]
@@ -537,39 +474,11 @@ sepref_definition vmtf_mark_to_rescore_also_reasons_fast_code
   unfolding isa_vmtf_mark_to_rescore_also_reasons_def PR_CONST_def
   unfolding while_eq_nfoldli[symmetric]
   apply (subst while_upt_while_direct, simp)
-  apply (rewrite at \<open>(\<hole>, _)\<close> zero_uint32_nat_def[symmetric])
-  unfolding one_uint32_nat_def[symmetric] nres_monad3 zero_uint64_nat_def[symmetric]
+  apply (annot_snat_const "TYPE(64)")
+  unfolding  nres_monad3 case_option_split
   by sepref
 
 declare vmtf_mark_to_rescore_also_reasons_fast_code.refine[sepref_fr_rules]
 
-
-sepref_definition vmtf_find_next_undef_fast_code
-  is \<open>uncurry (isa_vmtf_find_next_undef)\<close>
-  :: \<open>vmtf_remove_conc\<^sup>k *\<^sub>a trail_pol_fast_assn\<^sup>k \<rightarrow>\<^sub>a option_assn uint32_nat_assn\<close>
-  supply [[goals_limit=1]]
-  supply not_is_None_not_None[simp]
-  unfolding isa_vmtf_find_next_undef_def PR_CONST_def
-  apply (rewrite at \<open>WHILE\<^sub>T\<^bsup>_\<^esup> (\<lambda> _ . \<hole>) _ _\<close> short_circuit_conv)
-  by sepref
-
-declare vmtf_find_next_undef_code.refine[sepref_fr_rules]
-  vmtf_find_next_undef_fast_code.refine[sepref_fr_rules]
-
-
-sepref_register vmtf_find_next_undef_upd
-
-sepref_definition vmtf_find_next_undef_upd_fast_code
-  is \<open>uncurry isa_vmtf_find_next_undef_upd\<close>
-  :: \<open>trail_pol_fast_assn\<^sup>d *\<^sub>a vmtf_remove_conc\<^sup>d \<rightarrow>\<^sub>a
-     (trail_pol_fast_assn *a vmtf_remove_conc) *a
-        option_assn uint32_nat_assn\<close>
-  supply [[goals_limit=1]]
-  supply not_is_None_not_None[simp]
-  unfolding isa_vmtf_find_next_undef_upd_def PR_CONST_def
-  by sepref
-
-declare
-  vmtf_find_next_undef_upd_fast_code.refine[sepref_fr_rules]
 
 end
